src/lake/Lake/Build/Job/Monad.lean
@@ -102,13 +102,13 @@ example : MonadLiftT SpawnM FetchM := inferInstance
 namespace Job
 
 @[inline] def bindTask
-  [Monad m] [DataKind β]
+  [Monad m] [OptDataKind β]
   (f : JobTask α → m (JobTask β)) (self : Job α)
 : m (Job β) := return {self with task := ← f self.task, kind := inferInstance}
 
 /-- Spawn a job that asynchronously performs `act`. -/
 @[inline] protected def async
-  [DataKind α] (act : JobM α) (prio := Task.Priority.default) (caption := "")
+  [OptDataKind α] (act : JobM α) (prio := Task.Priority.default) (caption := "")
 : SpawnM (Job α) := fun fetch stack store ctx => .ofTask (caption := caption) <$> do
   BaseIO.asTask (prio := prio) do (withLoggedIO act) fetch stack store ctx {}
 
@@ -134,7 +134,7 @@ Logs the job's log and throws if there was an error.
 
 /-- Apply `f` asynchronously to the job's output. -/
 protected def mapM
-  [DataKind β] (self : Job α) (f : α → JobM β)
+  [OptDataKind β] (self : Job α) (f : α → JobM β)
   (prio := Task.Priority.default) (sync := false)
 : SpawnM (Job β) :=
   fun fetch stack store ctx trace => do
@@ -147,7 +147,7 @@ protected def mapM
 
 @[deprecated Job.mapM (since := "2024-12-06")]
 protected abbrev bindSync
-  [DataKind β] (self : Job α) (f : α → JobM β)
+  [OptDataKind β] (self : Job α) (f : α → JobM β)
   (prio := Task.Priority.default) (sync := false)
 : SpawnM (Job β) := self.mapM f prio sync
 
@@ -156,7 +156,7 @@ Apply `f` asynchronously to the job's output
 and asynchronously await the resulting job.
 -/
 def bindM
-  [DataKind β] (self : Job α) (f : α → JobM (Job β))
+  [OptDataKind β] (self : Job α) (f : α → JobM (Job β))
   (prio := Task.Priority.default) (sync := false)
 : SpawnM (Job β) :=
   fun fetch stack store ctx trace => do
@@ -174,7 +174,7 @@ def bindM
 
 @[deprecated bindM (since := "2024-12-06")]
 protected abbrev bindAsync
-  [DataKind β] (self : Job α) (f : α → SpawnM (Job β))
+  [OptDataKind β] (self : Job α) (f : α → SpawnM (Job β))
   (prio := Task.Priority.default) (sync := false)
 : SpawnM (Job β) := self.bindM (fun a => f a) prio sync
 
@@ -183,7 +183,7 @@ protected abbrev bindAsync
 results of `a` and `b`. The job `c` errors if either `a` or `b` error.
 -/
 @[inline] def zipResultWith
-  [DataKind γ] (f : JobResult α → JobResult β → JobResult γ) (self : Job α) (other : Job β)
+  [OptDataKind γ] (f : JobResult α → JobResult β → JobResult γ) (self : Job α) (other : Job β)
   (prio := Task.Priority.default) (sync := true)
 : Job γ := Job.ofTask $
   self.task.bind (prio := prio) (sync := true) fun rx =>
@@ -195,7 +195,7 @@ results of `a` and `b`. The job `c` errors if either `a` or `b` error.
 results of `a` and `b`. The job `c` errors if either `a` or `b` error.
 -/
 @[inline] def zipWith
-  [DataKind γ] (f : α → β → γ) (self : Job α) (other : Job β)
+  [OptDataKind γ] (f : α → β → γ) (self : Job α) (other : Job β)
   (prio := Task.Priority.default) (sync := true)
 : Job γ :=
   self.zipResultWith (other := other) (prio := prio) (sync := sync) fun
@@ -204,7 +204,7 @@ results of `a` and `b`. The job `c` errors if either `a` or `b` error.
 
 /-- Merges this job with another, discarding its output and trace. -/
 def add (self : Job α) (other : Job β) : Job α :=
-  have : DataKind α := self.kind
+  have : OptDataKind α := self.kind
   self.zipResultWith (other := other) fun
   | .ok a sa, .ok _ sb => .ok a {sa.merge sb with trace := sa.trace}
   | ra, rb => .error 0 {ra.state.merge rb.state with trace := ra.state.trace}
@@ -254,27 +254,27 @@ abbrev nil : BuildJob Unit :=
   Job.pure ()
 
 @[deprecated Job.map (since := "2024-12-06")]
-protected abbrev pure [DataKind α] (a : α) : BuildJob α :=
+protected abbrev pure [OptDataKind α] (a : α) : BuildJob α :=
   Job.pure a
 
 instance : Pure BuildJob := ⟨Job.pure⟩
 
 @[deprecated Job.map (since := "2024-12-06")]
-protected abbrev map [DataKind β] (f : α → β) (self : BuildJob α) : BuildJob β :=
+protected abbrev map [OptDataKind β] (f : α → β) (self : BuildJob α) : BuildJob β :=
   self.toJob.map f
 
 instance : Functor BuildJob where
   map := Job.map
 
 @[inline, deprecated "Removed without replacement." (since := "2024-12-06")]
-def mapWithTrace [DataKind β] (f : α → BuildTrace → β × BuildTrace) (self : BuildJob α) : BuildJob β :=
+def mapWithTrace [OptDataKind β] (f : α → BuildTrace → β × BuildTrace) (self : BuildJob α) : BuildJob β :=
   self.toJob.mapOk fun a s =>
     let (b, trace) := f a s.trace
     .ok b {s with trace}
 
 @[inline, deprecated Job.mapM (since := "2024-12-06")]
 protected def bindSync
-  [DataKind β] (self : BuildJob α) (f : α → BuildTrace → JobM (β × BuildTrace))
+  [OptDataKind β] (self : BuildJob α) (f : α → BuildTrace → JobM (β × BuildTrace))
   (prio : Task.Priority := .default) (sync := false)
 : SpawnM (Job β) :=
   self.toJob.mapM (prio := prio) (sync := sync) fun a => do
@@ -284,7 +284,7 @@ protected def bindSync
 
 @[inline, deprecated Job.bindM (since := "2024-12-06")]
 protected def bindAsync
-  [DataKind β] (self : BuildJob α) (f : α → BuildTrace → SpawnM (Job β))
+  [OptDataKind β] (self : BuildJob α) (f : α → BuildTrace → SpawnM (Job β))
   (prio : Task.Priority := .default) (sync := false)
  : SpawnM (Job β)  :=
   self.toJob.bindM (prio := prio) (sync := sync) fun a => do
@@ -312,7 +312,7 @@ abbrev mixArray (jobs : Array (BuildJob α)) : Id (BuildJob Unit) :=
 
 @[deprecated Job.zipWith (since := "2024-12-06")]
 abbrev zipWith
-  [DataKind γ] (f : α → β → γ) (self : BuildJob α) (other : BuildJob β)
+  [OptDataKind γ] (f : α → β → γ) (self : BuildJob α) (other : BuildJob β)
 : BuildJob γ :=
   self.toJob.zipWith f other.toJob
 
